more

compiler/src/compiler/SmallStep.v
@@ -8,11 +8,6 @@ Section step.
   Context (State : Type) (step : State -> (State -> Prop) -> Prop).
   Context {width: Z} {BW: Bitwidth width} {word: word.word width} {mem: map.map word byte}.
 
-  Inductive AEP :=
-  | AEP_A : (nat -> AEP) -> AEP
-  | AEP_E : (nat -> AEP) -> AEP
-  | AEP_P : (State -> Prop) -> AEP.
-  
   Definition State' : Type := State * AEP.
   Inductive step' : State' -> (State' -> Prop) -> Prop :=
   | step_usual s1 aep P : step s1 (fun s2 => P (s2, aep)) ->
@@ -24,24 +19,36 @@ Section step.
 
   Fixpoint post_of aep :=
     match aep with
-    | AEP_A aep' => fun s => forall n, runsTo step s (post_of (aep' n))
-    | AEP_E aep' => fun s => exists n, runsTo step s (post_of (aep' n))
-    | AEP_P P => P
+    | AEP_A aep' => fun post => fun s => forall n, runsTo step s (post_of (aep' n) post)
+    | AEP_E aep' => fun post => fun s => exists n, runsTo step s (post_of (aep' n) post)
+    | AEP_P X => fun post => fun s' => post X s'
     end.
 
-  Lemma step'_to_step s aep : runsTo step' (s, aep)
+  Lemma step_impl_step' s aep post :
+    runsTo step s post ->
+    runsTo step' (s, aep) (fun '(s', aep') => post s' /\ aep' = aep).
+  Proof.
+    intros H. induction H.
+    - apply runsToDone. auto.
+    - eapply runsTo_weaken.
+      { apply runsToStep_cps. apply step_usual. eapply weaken_step. 2: eassumption.
+        eassumption. }
+      simpl. auto.
+  Qed.
+  
+  Lemma step'_to_step s aep post : runsTo step' (s, aep)
                                 (fun '(s', aep') =>
                                    match aep' with
-                                   | AEP_P P => P s'
+                                   | AEP_P P => post P s'
                                    | _ => False
                                    end) <->
-                                runsTo step s (post_of aep).
+                                runsTo step s (post_of aep post).
   Proof.
     split.
-    - intros H. remember (fun _ => _) as post.
-      eassert (forall s, post s -> _) as X.
+    - intros H. remember (fun _ => _) as post'.
+      eassert (forall s, post' s -> _) as X.
       { intros. subst. apply H0. }
-      clear Heqpost. revert X.
+      clear Heqpost'. revert X.
       remember (s, aep) as s_aep. replace s with (fst s_aep) by (subst; reflexivity).
       replace aep with (snd s_aep) by (subst; reflexivity). clear Heqs_aep.
       induction H; intros X.
@@ -51,8 +58,9 @@ Section step.
         simpl. inversion H; subst.
         -- eapply runsToStep. 1: eassumption. simpl. intros. apply H1 in H2. apply H2.
         -- apply runsToDone. simpl. intros. specialize (H5 n). apply H1 in H5. apply H5.         -- apply runsToDone. destruct H5 as [x H5]. simpl. exists x. apply H1 in H5. apply H5.
-    - intros H. remember (post_of _) as post.
-      assert (Hpost : forall s, post s -> post_of aep s) by (subst; auto).
-      clear Heqpost. revert aep Hpost. induction H; intros aep Hpost.
-      + induction aep.
-        -- apply runsToStep_cps. apply step_A. intros. apply H0. simpl in *.
+    - intros H. remember (post_of _ _) as post'.
+      assert (Hpost' : forall s, post' s -> post_of aep post s) by (subst; auto).
+      clear Heqpost'. revert aep Hpost'. induction H; intros aep Hpost.
+      + apply Hpost in H. clear Hpost P. induction aep.
+        -- apply runsToStep_cps. apply step_A. intros x. simpl in H. specialize (H x).
+           specialize (H0 x). apply runsTo_trans_cps. apply runsTo_weaken. apply step_impl_step'. apply step_A. intros. apply H0. simpl in *.
